Nary.v
@@ -10,6 +10,69 @@ Import ListNotations.
 (** For function of arity [n], we re-use [NaryFunctions.nfun A n B]
     and its notation [A^^n-->B]. *)
 
+Arguments ncurry {A B n}.
+Arguments nuncurry {A B n}.
+Arguments nprod_to_list {A n}.
+Arguments nfun_to_nfun {A B C} f {n}.
+
+Lemma nuncurry_ncurry {A B n} (f : A^n->B) (v:A^n) :
+  nuncurry (ncurry f) v = f v.
+Proof.
+ induction n; cbn in *; auto.
+ - now destruct v.
+ - destruct v as (a,v). now rewrite IHn.
+Qed.
+
+Lemma nprod_to_list_length {A} n (v:A^n) :
+ length (nprod_to_list v) = n.
+Proof.
+ induction n; cbn; auto. destruct v; cbn; auto.
+Qed.
+
+Fixpoint nprod_map {A B} (f:A->B) {n} : A^n -> B^n :=
+  match n with
+  | 0 => fun _ => tt
+  | S n => fun '(a,v) => (f a, nprod_map f v)
+  end.
+
+Lemma nprod_map_to_list {A B} (f:A->B) {n} (v:A^n) :
+ nprod_to_list (nprod_map f v) = map f (nprod_to_list v).
+Proof.
+ induction n; cbn; destruct v; cbn; f_equal; auto.
+Qed.
+
+(** A variant of [nprod_of_list] with a precise size as target *)
+
+Fixpoint optnprod {A} n (l:list A) : option (A^n) :=
+ match n, l return option (A^n) with
+ | 0, []  => Some tt
+ | S n, x::l => option_map (pair x) (optnprod n l)
+ | _, _ => None
+ end.
+
+Lemma optnprod_some {A} n (l:list A) :
+  optnprod n l <> None <-> length l = n.
+Proof.
+ revert l. induction n; destruct l; cbn; try easy.
+ specialize (IHn l).
+ destruct (optnprod n l); cbn in *; intuition; try easy.
+ f_equal. now apply H.
+Qed.
+
+Lemma optnprod_to_list {A} n (l:list A) (v:A^n) :
+ optnprod n l = Some v <-> nprod_to_list v = l.
+Proof.
+ revert l. induction n; destruct l; cbn in *.
+ - now destruct v.
+ - now intuition.
+ - now intuition.
+ - destruct v as (b,v). specialize (IHn v l).
+   destruct (optnprod n l); cbn.
+   + split; intros [= <- <-]; f_equal. now apply IHn.
+     intuition. congruence.
+   + split. easy. intros [= <- <-]. now intuition.
+Qed.
+
 (** Then, a compact alternative to [option { n:nat & A^^n-->B }] *)
 
 Inductive optnfun A B :=
@@ -25,64 +88,14 @@ Definition get_arity {A B} (f : optnfun A B) :=
  | NFun n _ => Some n
  end.
 
-Fixpoint mk_nprod {A} n (l:list A)(dft:A) : A^n :=
- match n, l return A^n with
- | 0, _  => tt
- | S n, [] => (dft, mk_nprod n l dft)
- | S n, x::l => (x, mk_nprod n l dft)
- end.
-
-Definition build_args {A B} :=
-  fix build {n} (l : list A)(dft:B) : A^^n-->B -> B :=
-    match n, l with
-    | 0, [] => fun f => f
-    | S n, a :: l => fun f => build l dft (f a)
-    | _, _ => fun _ => dft
-    end.
-
-Definition optnapply {A B}(f:optnfun A B)(l:list A)(dft:B) :=
+Definition optnapply {A B}(f:optnfun A B)(l:list A) :=
  match f with
- | NFun _ f => build_args l dft f
- | Nop => dft
+ | NFun n f => option_map (nuncurry f) (optnprod n l)
+ | Nop => None
  end.
 
-Arguments nfun_to_nfun {A B C} f {n}.
-Arguments ncurry {A B n}.
-Arguments nuncurry {A B n}.
-Arguments nprod_to_list {A n}.
-
-Lemma build_args_ntn {A B B' n} (l : list A)(f:B->B')(any:B)(any':B') :
- length l = n ->
- forall (a : A^^n-->B),
- build_args l any' (nfun_to_nfun f a) = f (build_args l any a).
-Proof.
- intros <-. induction l; simpl; auto.
-Qed.
-
-Lemma to_nprod {A} n (l:list A) :
-  length l = n -> exists v : A^n, nprod_to_list v = l.
-Proof.
- intros <-.
- exists (nprod_of_list _ l). induction l; cbn; f_equal; auto.
-Qed.
-
-Lemma nprod_to_list_length {A} n (v:A^n) :
- length (nprod_to_list v) = n.
-Proof.
- induction n; cbn; auto. destruct v; cbn; auto.
-Qed.
-
-Lemma build_args_nprod {A B} n (v:A^n) (f:A^^n-->B) (dft:B) :
-  build_args (nprod_to_list v) dft f = nuncurry f v.
-Proof.
- induction n; cbn in *; auto.
- destruct v as (a,v). apply IHn.
-Qed.
-
-Lemma nuncurry_ncurry {A B n} (f : A^n->B) (v:A^n) :
-  nuncurry (ncurry f) v = f v.
-Proof.
- induction n; cbn in *; auto.
- - now destruct v.
- - destruct v as (a,v). now rewrite IHn.
-Qed.
+Definition napply_dft {A B}(f:optnfun A B)(l:list A)(dft:B) :=
+ match optnapply f l with
+ | Some b => b
+ | None => dft
+ end.
